Source/DafnyCompilers/CSharp/Compiler.dfy
@@ -3,23 +3,122 @@ include "../CSharpCompat.dfy"
 
 // import opened CSharpSystem
 
+module Utils {
+  function method SeqMap<T, Q>(f: T ~> Q, ts: seq<T>) : seq<Q>
+    reads * // FIXME
+    requires forall t | t in ts :: f.requires(t)
+  {
+    if ts == [] then [] else [f(ts[0])] + SeqMap(f, ts[1..])
+  }
+}
+
 module {:extern "Microsoft.Dafny.Compilers.SelfHosting.CSharp"} CSharpDafnyCompiler {
   import System
   import CSharpDafnyAST
+  import opened CSharpUtils
   import opened Microsoft.Dafny
+  import Utils
+
+  module AST {
+    datatype Expression =
+      | StringLiteralExpr(str: string)
+      | InvalidExpression
+
+    datatype Stmt =
+      | PrintStmt(stmts: seq<Expression>)
+      | InvalidStmt
+
+    type BlockStmt = seq<Stmt>
+
+    datatype Method = Method(methodBody: BlockStmt)
+
+    datatype Program = Program(mainMethod: Method)
+  }
+
+  module Translator {
+    import AST
+    import Utils
+    import opened CSharpUtils
+    import CSharpDafnyAST
+
+    function method TranslateExpression(s: CSharpDafnyAST.Expression) : AST.Expression reads * {
+      if s is CSharpDafnyAST.StringLiteralExpr then
+        var p := s as CSharpDafnyAST.StringLiteralExpr;
+        if p.Value is System.String then
+          AST.StringLiteralExpr(StringUtils.OfCString(p.Value as System.String))
+        else
+          AST.InvalidExpression
+      else AST.InvalidExpression
+    }
+
+    function method TranslateStatement(s: CSharpDafnyAST.Statement) : AST.Stmt reads * {
+      if s is CSharpDafnyAST.PrintStmt then
+        var p := s as CSharpDafnyAST.PrintStmt;
+        AST.PrintStmt(Utils.SeqMap(TranslateExpression, ListUtils.ToSeq(p.Args)))
+      else AST.InvalidStmt
+    }
+
+    function method TranslateBlock(b: CSharpDafnyAST.BlockStmt) : AST.BlockStmt reads * {
+      Utils.SeqMap(TranslateStatement, ListUtils.ToSeq(b.Body))
+    }
+
+    function method TranslateMethod(m: CSharpDafnyAST.Method) : AST.Method reads * {
+      AST.Method(TranslateBlock(m.methodBody))
+    }
+
+    function method TranslateProgram(p: CSharpDafnyAST.Program) : AST.Program reads * {
+      AST.Program(TranslateMethod(p.MainMethod))
+    }
+  }
+
+  module Compiler {
+    import opened AST
+
+    class CSharpAST {}
+
+    function method CompileExpression(s: Expression) : CSharpAST? {
+      match s {
+        case StringLiteralExpr(str) => null
+        case InvalidExpression => null
+      }
+    }
+
+    function method CompileStmt(s: Stmt) : CSharpAST? {
+      match s {
+        case PrintStmt(stmts) => null
+        case InvalidStmt => null
+      }
+    }
+
+    function method CompileMethod(m: Method) : CSharpAST? {
+      match m {
+        case Method(methodBody) => null
+      }
+    }
+
+    function method CompileProgram(p: Program) : CSharpAST? {
+      match p {
+        case Program(mainMethod) => CompileMethod(mainMethod)
+      }
+    }
+  }
+
+  method WriteStr(output: ConcreteSyntaxTree, str: string) {
+    output.Write(StringUtils.ToCString(str));
+  }
 
   class {:extern} DafnyCSharpCompiler {
     constructor() {
     }
 
-    method Compile(dafnyProgram: CSharpDafnyAST.Program, output: ConcreteSyntaxTree)
-    {
-
+    method Compile(dafnyProgram: CSharpDafnyAST.Program,
+                   output: ConcreteSyntaxTree) {
+      WriteStr(output, "Console.WriteLine(\"Hello, world!\")");
     }
 
     method EmitCallToMain(mainMethod: CSharpDafnyAST.Method,
-      baseName: System.String,
-      output: ConcreteSyntaxTree) {
+                          baseName: System.String,
+                          output: ConcreteSyntaxTree) {
     }
   }
 }
